parser/LLPrediction_error_free.v
@@ -28,16 +28,18 @@ Module LLPredictionErrorFreeFn (Import D : Defs.T).
     forall sp, In sp sps -> stable_config sp.(stack).
 
   Lemma cstep_never_returns_SpInvalidState :
-    forall g av sp,
+    forall g pm av sp,
       suffix_stack_wf g sp.(stack)
-      -> cstep g av sp <> CstepError SpInvalidState.
+      -> cstep g pm av sp <> CstepError SpInvalidState.
   Proof.
-    intros g av sp hw; unfold not; intros hs.
+    intros g pm av sp hw; unfold not; intros hs.
     unfold cstep in hs; dms; tc; inv hw.
   Qed.
 
   Lemma llc_never_returns_SpInvalidState :
     forall (g    : grammar)
+           (pm   : production_map)
+           (hc   : production_map_correct pm g)
            (pair : nat * nat)
            (a    : Acc lex_nat_pair pair)
            (av   : NtSet.t)
@@ -45,9 +47,9 @@ Module LLPredictionErrorFreeFn (Import D : Defs.T).
            (a'   : Acc lex_nat_pair (meas g av sp)),
       pair = meas g av sp
       -> suffix_stack_wf g sp.(stack)
-      -> llc g av sp a' <> inl SpInvalidState.
+      -> llc hc av sp a' <> inl SpInvalidState.
   Proof.
-    intros g pair a'.
+    intros g pm hc pair a'.
     induction a' as [pair hlt IH].
     intros av sp a heq hw; unfold not; intros hs; subst.
     apply llc_error_cases in hs.
@@ -62,11 +64,11 @@ Module LLPredictionErrorFreeFn (Import D : Defs.T).
   Qed.
   
   Lemma llClosure_never_returns_SpInvalidState :
-    forall g sps,
+    forall g pm (hc : production_map_correct pm g) sps,
       all_suffix_stacks_wf g sps
-      -> llClosure g sps <> inl SpInvalidState.
+      -> llClosure hc sps <> inl SpInvalidState.
   Proof.
-    intros g sps hw; unfold not; intros hc.
+    intros g pm hpc sps hw; unfold not; intros hc.
     unfold llClosure in hc.
     apply aggrClosureResults_error_in_input in hc.
     apply in_map_iff in hc; destruct hc as [sp [hs hi]].
@@ -75,12 +77,12 @@ Module LLPredictionErrorFreeFn (Import D : Defs.T).
   Qed.
 
   Lemma llStartState_never_returns_SpInvalidState :
-    forall g fr frs o x suf,
+    forall g pm (hc : production_map_correct pm g) fr frs o x suf,
       suffix_stack_wf g (fr, frs)
       -> fr = SF o (NT x :: suf)
-      -> llStartState g x (fr, frs) <> inl SpInvalidState.
+      -> llStartState hc x (fr, frs) <> inl SpInvalidState.
   Proof.
-    intros g fr frs o x suf hw heq; unfold not; intros hss.
+    intros g pm hc fr frs o x suf hw heq; unfold not; intros hss.
     eapply llClosure_never_returns_SpInvalidState; eauto.
     intros sp hi.
     unfold llInitSps in hi.
@@ -90,9 +92,9 @@ Module LLPredictionErrorFreeFn (Import D : Defs.T).
     clear hss.
     inv hw; sis; subst.
     - wf_upper_nil. 
-      apply rhssForNt_in_iff; eauto.
+      eapply rhssFor_in_iff; eauto.
     - wf_upper_nil. 
-      apply rhssForNt_in_iff; auto.
+      eapply rhssFor_in_iff; eauto.
   Qed.
 
   Lemma handleFinalSubparsers_never_returns_error :
@@ -155,14 +157,14 @@ Module LLPredictionErrorFreeFn (Import D : Defs.T).
   Qed.
 
   Lemma llc_preserves_suffix_stack_wf_invar :
-    forall g pr (a : Acc lex_nat_pair pr) av sp sp' a' sps',
+    forall g pm (hc : production_map_correct pm g) pr (a : Acc lex_nat_pair pr) av sp sp' a' sps',
       pr = meas g av sp
       -> suffix_stack_wf g sp.(stack)
-      -> llc g av sp a' = inr sps'
+      -> llc hc av sp a' = inr sps'
       -> In sp' sps'
       -> suffix_stack_wf g sp'.(stack).
   Proof.
-    intros g pr a'.
+    intros g pm hc pr a'.
     induction a' as [pr hlt IH]; intros av sp sp' a sps' heq hw hs hi; subst.
     apply llc_success_cases in hs.
     destruct hs as [[hd heq] | [sps'' [av' [hs [crs [heq heq']]]]]]; subst.
@@ -177,12 +179,12 @@ Module LLPredictionErrorFreeFn (Import D : Defs.T).
   Qed.
   
   Lemma llClosure_preserves_suffix_stack_wf_invar :
-    forall g sps sps',
+    forall g pm (hc : production_map_correct pm g) sps sps',
       all_suffix_stacks_wf g sps
-      -> llClosure g sps = inr sps'
+      -> llClosure hc sps = inr sps'
       -> all_suffix_stacks_wf g sps'.
   Proof.
-    intros g sps sps' ha hc.
+    intros g pm hpc sps sps' ha hc.
     unfold llClosure in hc.
     unfold all_suffix_stacks_wf.
     intros sp' hi.
@@ -195,24 +197,24 @@ Module LLPredictionErrorFreeFn (Import D : Defs.T).
   Qed.
 
   Lemma cstepDone_stable_config :
-    forall g av sp,
+    forall g pm av sp,
       suffix_stack_wf g sp.(stack)
-      -> cstep g av sp = CstepDone
+      -> cstep g pm av sp = CstepDone
       -> stable_config sp.(stack).
   Proof.
-    intros g av sp hw hs.
+    intros g pm av sp hw hs.
     unfold cstep in hs; dms; tc; sis; inv hw; auto.
   Qed.
 
   Lemma sp_in_llc_result_stable_config :
-    forall g pr (a : Acc lex_nat_pair pr) av sp sp' a' sps',
+    forall g pm (hc : production_map_correct pm g) pr (a : Acc lex_nat_pair pr) av sp sp' a' sps',
       pr = meas g av sp
       -> suffix_stack_wf g sp.(stack)
-      -> llc g av sp a' = inr sps'
+      -> llc hc av sp a' = inr sps'
       -> In sp' sps'
       -> stable_config sp'.(stack).
   Proof.
-    intros g pr a'.
+    intros g pm hc pr a'.
     induction a' as [pr hlt IH]; intros av sp sp' a sps' heq hw hs hi; subst.
     apply llc_success_cases in hs.
     destruct hs as [[hd heq] | [sps'' [av' [hs [crs [heq heq']]]]]]; subst.
@@ -228,12 +230,12 @@ Module LLPredictionErrorFreeFn (Import D : Defs.T).
   Qed.
 
   Lemma all_stacks_stable_after_closure :
-    forall g sps sps',
+    forall g pm (hc : production_map_correct pm g) sps sps',
       all_suffix_stacks_wf g sps
-      -> llClosure g sps = inr sps'
+      -> llClosure hc sps = inr sps'
       -> all_stacks_stable sps'.
   Proof.
-    intros g sps sps' hw hc.
+    intros g pm hpc sps sps' hw hc.
     unfold llClosure in hc.
     unfold all_stacks_stable.
     intros sp' hi.
@@ -246,49 +248,49 @@ Module LLPredictionErrorFreeFn (Import D : Defs.T).
   Qed.
 
   Lemma llTarget_never_returns_SpInvalidState :
-    forall g a sps,
+    forall g pm (hc : production_map_correct pm g) a sps,
       all_suffix_stacks_wf g sps
       -> all_stacks_stable sps
-      -> llTarget g a sps <> inl SpInvalidState.
+      -> llTarget hc a sps <> inl SpInvalidState.
   Proof.
-    intros g a sps hw hs; unfold not; intros ht; unfold llTarget in ht; dmeq hm.
+    intros g pm hc a sps hw hs; unfold not; intros ht; unfold llTarget in ht; dmeq hm.
     - inv ht; eapply move_never_returns_SpInvalidState_for_ready_sps; eauto.
     - eapply move_preserves_suffix_stack_wf_invar in hm; eauto.
       dmeq hc; tc; inv ht; eapply llClosure_never_returns_SpInvalidState; eauto.
   Qed.
 
   Lemma llTarget_preserves_suffix_stacks_wf_invar :
-    forall g a sps sps',
+    forall g pm (hc : production_map_correct pm g) a sps sps',
       all_suffix_stacks_wf g sps
-      -> llTarget g a sps = inr sps'
+      -> llTarget hc a sps = inr sps'
       -> all_suffix_stacks_wf g sps'.
   Proof.
-    intros g a sps sps' hw ht; unfold llTarget in ht.
+    intros g pm hc a sps sps' hw ht; unfold llTarget in ht.
     dmeq hm; tc; dmeq hc; tc; inv ht.
     eapply move_preserves_suffix_stack_wf_invar in hm; eauto.
     eapply llClosure_preserves_suffix_stack_wf_invar; eauto.
   Qed.
 
   Lemma llTarget_preserves_stacks_stable_invar :
-    forall g a sps sps',
+    forall g pm (hc : production_map_correct pm g) a sps sps',
       all_suffix_stacks_wf g sps
       -> all_stacks_stable sps
-      -> llTarget g a sps = inr sps'
+      -> llTarget hc a sps = inr sps'
       -> all_stacks_stable sps'.
   Proof.
-    intros g a sps sps' hw hs ht; unfold llTarget in ht.
+    intros g pm hc a sps sps' hw hs ht; unfold llTarget in ht.
     dmeq hm; tc; dmeq hc; tc; inv ht.
     eapply move_preserves_suffix_stack_wf_invar in hm; eauto.
     eapply all_stacks_stable_after_closure; eauto.
   Qed.
 
   Lemma llPredict'_never_returns_SpInvalidState :
-    forall g ts sps,
+    forall g pm (hc : production_map_correct pm g) ts sps,
       all_suffix_stacks_wf g sps
       -> all_stacks_stable sps
-      -> llPredict' g sps ts <> PredError SpInvalidState.
+      -> llPredict' hc sps ts <> PredError SpInvalidState.
   Proof.
-    intros g ts; induction ts as [| (a,l) ts IH]; intros sps ha ha';
+    intros g pm hc ts; induction ts as [| (a,l) ts IH]; intros sps ha ha';
       unfold not; intros hl; sis.
     - eapply handleFinalSubparsers_never_returns_error; eauto.
     - destruct sps as [| sp sps']; tc.
@@ -300,37 +302,37 @@ Module LLPredictionErrorFreeFn (Import D : Defs.T).
   Qed.
 
   Lemma llStartState_preserves_stacks_wf_invar :
-    forall g fr frs o x suf sps,
+    forall g pm (hc : production_map_correct pm g) fr frs o x suf sps,
       suffix_stack_wf g (fr, frs)
       -> fr = SF o (NT x :: suf)
-      -> llStartState g x (fr, frs) = inr sps
+      -> llStartState hc x (fr, frs) = inr sps
       -> all_suffix_stacks_wf g sps.
   Proof.
-    intros g [suf'] frs o x suf sps hw heq hs; sis; subst.
+    intros g pm hc [suf'] frs o x suf sps hw heq hs; sis; subst.
     eapply llClosure_preserves_suffix_stack_wf_invar; eauto.
     unfold all_suffix_stacks_wf; intros sp hi.
     eapply llInitSps_preserves_suffix_stack_wf_invar; eauto.
   Qed.
 
   Lemma llStartState_all_stacks_stable :
-    forall g cr o x suf frs sps,
+    forall g pm (hc : production_map_correct pm g) cr o x suf frs sps,
       cr = SF o (NT x :: suf)
       -> suffix_stack_wf g (cr, frs)
-      -> llStartState g x (cr, frs) = inr sps
+      -> llStartState hc x (cr, frs) = inr sps
       -> all_stacks_stable sps.
   Proof.
-    intros g cr o x suf frs sps ? hw hs sp hi.
+    intros g pm hc cr o x suf frs sps ? hw hs sp hi.
     eapply all_stacks_stable_after_closure; eauto.
     eapply llInitSps_preserves_suffix_stack_wf_invar; eauto.
   Qed.
 
   Lemma llPredict_never_returns_SpInvalidState :
-    forall g fr frs o x suf ts,
+    forall g pm (hc : production_map_correct pm g) fr frs o x suf ts,
       suffix_stack_wf g (fr, frs)
       -> fr = SF o (NT x :: suf)
-      -> llPredict g x (fr, frs) ts <> PredError SpInvalidState.
+      -> llPredict hc x (fr, frs) ts <> PredError SpInvalidState.
   Proof.
-    intros g fr frs o x suf ts hw heq; unfold not; intros hl.
+    intros g pm hc fr frs o x suf ts hw heq; unfold not; intros hl.
     unfold llPredict in hl.
     dmeq hss.
     - inv hl.
@@ -343,14 +345,14 @@ Module LLPredictionErrorFreeFn (Import D : Defs.T).
   (* LEFT RECURSION CASE *)
 
   Lemma cstep_LeftRecursion_facts :
-    forall g av pred fr frs x,
-      cstep g av (Sp pred (fr, frs)) = CstepError (SpLeftRecursion x)
+    forall g pm av pred fr frs x,
+      cstep g pm av (Sp pred (fr, frs)) = CstepError (SpLeftRecursion x)
       -> ~ NtSet.In x av
          /\ NtSet.In x (allNts g)
          /\ exists o suf,
              fr = SF o (NT x :: suf).
   Proof.
-    intros g av pred fr frs x hs.
+    intros g pm av pred fr frs x hs.
     unfold cstep in hs; repeat dmeq h; tc; inv hs; sis.
     repeat split; eauto.
     - unfold not; intros hi.
@@ -359,12 +361,12 @@ Module LLPredictionErrorFreeFn (Import D : Defs.T).
   Qed.
 
   Lemma cstep_never_finds_left_recursion :
-    forall g av sp x,
+    forall g pm av sp x,
       no_left_recursion g
       -> unavailable_nts_invar g av sp
-      -> cstep g av sp <> CstepError (SpLeftRecursion x).
+      -> cstep g pm av sp <> CstepError (SpLeftRecursion x).
   Proof.
-    intros g av [pred (fr, frs)] x hn hu; unfold not; intros hs.
+    intros g pm av [pred (fr, frs)] x hn hu; unfold not; intros hs.
     pose proof hs as hs'.
     apply cstep_LeftRecursion_facts in hs'.
     destruct hs' as [hn' [hi [o [suf' heq]]]]; subst.
@@ -375,13 +377,13 @@ Module LLPredictionErrorFreeFn (Import D : Defs.T).
   Qed.
 
   Lemma llc_never_finds_left_recursion :
-    forall g pr (a : Acc lex_nat_pair pr) av sp a' x,
+    forall g pm (hc : production_map_correct pm g) pr (a : Acc lex_nat_pair pr) av sp a' x,
       no_left_recursion g
       -> unavailable_nts_invar g av sp
       -> pr = meas g av sp
-      -> llc g av sp a' <> inl (SpLeftRecursion x).
+      -> llc hc av sp a' <> inl (SpLeftRecursion x).
   Proof.
-    intros g pr a'; induction a' as [pr hlt IH]. 
+    intros g pm hpc pr a'; induction a' as [pr hlt IH]. 
     intros av sp a x hn hu heq; unfold not; intros hs; subst.
     apply llc_error_cases in hs.
     destruct hs as [hs | [sps [av' [hs [crs [hc ha]]]]]]; subst.
@@ -395,11 +397,11 @@ Module LLPredictionErrorFreeFn (Import D : Defs.T).
   Qed.
 
   Lemma closure_never_finds_left_recursion :
-    forall g x sps,
+    forall g pm (hc : production_map_correct pm g) x sps,
       no_left_recursion g
-      -> llClosure g sps <> inl (SpLeftRecursion x).
+      -> llClosure hc sps <> inl (SpLeftRecursion x).
   Proof.
-    intros g x sps hn; unfold not; intros hc.
+    intros g pm hpc x sps hn; unfold not; intros hc.
     unfold llClosure in hc.
     apply aggrClosureResults_error_in_input in hc.
     apply in_map_iff in hc.
@@ -430,22 +432,22 @@ Module LLPredictionErrorFreeFn (Import D : Defs.T).
   Qed.
 
   Lemma llTarget_never_returns_SpLeftRecursion :
-    forall g a sps x,
+    forall g pm (hc : production_map_correct pm g) a sps x,
       no_left_recursion g
-      -> llTarget g a sps <> inl (SpLeftRecursion x).
+      -> llTarget hc a sps <> inl (SpLeftRecursion x).
   Proof.
-    intros g a sps x hn; unfold not; intros ht.
+    intros g pm hc a sps x hn; unfold not; intros ht.
     unfold llTarget in ht; dmeq hm; tc.
     - inv ht; eapply move_never_returns_SpLeftRecursion; eauto.
     - dmeq hc; tc; inv ht; eapply closure_never_finds_left_recursion; eauto.
   Qed.
   
   Lemma llPredict'_never_returns_SpLeftRecursion :
-    forall g ts sps x,
+    forall g pm (hc : production_map_correct pm g) ts sps x,
       no_left_recursion g
-      -> llPredict' g sps ts <> PredError (SpLeftRecursion x).
+      -> llPredict' hc sps ts <> PredError (SpLeftRecursion x).
   Proof.
-    intros g ts; induction ts as [| (a,l) ts IH];
+    intros g pm hc ts; induction ts as [| (a,l) ts IH];
       intros sps x hn; unfold not; intros hl; sis.
     - eapply handleFinalSubparsers_never_returns_error; eauto.
     - destruct sps as [| sp sps']; tc; dm; tc; dmeq hm; tc.
@@ -454,11 +456,11 @@ Module LLPredictionErrorFreeFn (Import D : Defs.T).
   Qed.
 
   Lemma llPredict_never_returns_SpLeftRecursion :
-    forall g x x' fr frs ts,
+    forall g pm (hc : production_map_correct pm g) x x' fr frs ts,
       no_left_recursion g
-      -> llPredict g x (fr, frs) ts <> PredError (SpLeftRecursion x').
+      -> llPredict hc x (fr, frs) ts <> PredError (SpLeftRecursion x').
   Proof.
-    intros g x x' fr frs ts hn hl; unfold llPredict in hl; dmeq hss.
+    intros g pm hc x x' fr frs ts hn hl; unfold llPredict in hl; dmeq hss.
     - inv hl; eapply closure_never_finds_left_recursion; eauto. 
     - eapply llPredict'_never_returns_SpLeftRecursion; eauto.
   Qed.
@@ -467,49 +469,49 @@ Module LLPredictionErrorFreeFn (Import D : Defs.T).
      types of prediction errors *)
 
   Lemma llTarget_never_returns_error :
-    forall g a sps e,
+    forall g pm (hc : production_map_correct pm g) a sps e,
       no_left_recursion g
       -> all_suffix_stacks_wf g sps
       -> all_stacks_stable sps
-      -> llTarget g a sps <> inl e.
+      -> llTarget hc a sps <> inl e.
   Proof.
-    unfold not; intros g a sps e hn hw hs hl; destruct e.
+    unfold not; intros g pm hc a sps e hn hw hs hl; destruct e.
     - eapply llTarget_never_returns_SpInvalidState ; eauto.
     - eapply llTarget_never_returns_SpLeftRecursion; eauto.
   Qed.
 
   Lemma llStartState_never_returns_error :
-    forall g fr frs o x suf e,
+    forall g pm (hc : production_map_correct pm g) fr frs o x suf e,
       no_left_recursion g
       -> suffix_stack_wf g (fr, frs)
       -> fr = SF o (NT x :: suf)
-      -> llStartState g x (fr, frs) <> inl e.
+      -> llStartState hc x (fr, frs) <> inl e.
   Proof.
-    intros ? ? ? ? ? ? e ? ? ?; unfold not; intros hs; subst; destruct e.
+    intros ? ? ? ? ? ? ? ? e ? ? ?; unfold not; intros hs; subst; destruct e.
     - eapply llStartState_never_returns_SpInvalidState; eauto.
     - eapply closure_never_finds_left_recursion; eauto.
   Qed.
 
   Lemma llPredict'_never_returns_error :
-    forall g sps ts e,
+    forall g pm (hc : production_map_correct pm g) sps ts e,
       no_left_recursion g
       -> all_suffix_stacks_wf g sps
       -> all_stacks_stable sps
-      -> llPredict' g sps ts <> PredError e.
+      -> llPredict' hc sps ts <> PredError e.
   Proof.
-    intros g sps ts e hn hw hs hl; destruct e.
+    intros g pm hc sps ts e hn hw hs hl; destruct e.
     - eapply llPredict'_never_returns_SpInvalidState ; eauto.
     - eapply llPredict'_never_returns_SpLeftRecursion; eauto.
   Qed.
   
   Lemma llPredict_never_returns_error :
-    forall g fr o x suf frs ts e,
+    forall g pm (hc : production_map_correct pm g) fr o x suf frs ts e,
       fr = SF o (NT x :: suf)
       -> no_left_recursion g
       -> suffix_stack_wf g (fr, frs)
-      -> llPredict g x (fr, frs) ts <> PredError e.
+      -> llPredict hc x (fr, frs) ts <> PredError e.
   Proof.
-    unfold not; intros g fr o x suf frs ts e ? hn hw hl; subst.
+    unfold not; intros g pm hc fr o x suf frs ts e ? hn hw hl; subst.
     destruct e as [| x'].
     - eapply llPredict_never_returns_SpInvalidState;  eauto.
     - eapply llPredict_never_returns_SpLeftRecursion; eauto.
